Hoare.thy
@@ -17,7 +17,7 @@ text {* Verification condition generator *}
 named_theorems hl_rules
 
 method hoare_init uses simp = 
-  ((rule allI | rule ballI | subst simp | subst fst_conv)+)?
+  ((rule allI | rule ballI | subst simp | subst fst_conv | subst snd_conv)+)?
 
 method hoare_step uses simp hl = 
   (hoare_init simp: simp, (assumption | rule subset_refl | rule hl hl_rules))
@@ -74,6 +74,7 @@ proof (simp add: ht_def cwhile_def seq_def)
     by auto
 qed
 
+
 (***********************************************************************************************)
 
 text {* Weakening / Strengthening / Consequence Rules *}
@@ -92,6 +93,9 @@ lemma hl_conseq: "\<forall>z. ht (P' z) c (Q' z) \<Longrightarrow> \<forall>s. s
 
 lemma hl_kleymann: "\<forall>z. ht (P' z) x (Q' z) \<Longrightarrow> \<forall>s t. (\<forall>z. s \<in> P' z \<longrightarrow> t \<in> Q' z) \<longrightarrow> (\<forall>z. s \<in> P z \<longrightarrow> t \<in> Q z) \<Longrightarrow> \<forall>z. ht (P z) x (Q z)"
   by (fastforce simp: apre_def seq_def ht_def)
+
+lemma hl_for [hl_rules]: "ht P (assign j_upd n) R \<Longrightarrow> ht ({s. j s \<le> m s} \<inter> R) x (subst R j_upd (\<lambda>s. j s + 1)) \<Longrightarrow> R \<inter> -{s. j s \<le> m s} \<subseteq> Q \<Longrightarrow>  ht P (cfor (j_upd, j) n m x) Q"
+  by (hoare simp: cfor_def hl: hl_while first: hl_post [where Q'="(-{s. j s \<le> m s} \<sqinter> R)"]) force
 
 (***********************************************************************************************)
 
@@ -125,6 +129,10 @@ lemma hl_rec [hl_rules]: "mono f \<Longrightarrow> (\<And>x. \<forall>z. ht (P z
 (***********************************************************************************************)
 
 text {* Annotated programs *}
+
+lemma hl_afor [hl_rules]: "ht P (assign j_upd n) R \<Longrightarrow> ht ({s. j s < m s} \<inter> R) x (subst R j_upd (\<lambda>s. j s + 1)) \<Longrightarrow> R \<inter> {s. j s = m s} \<subseteq> Q \<Longrightarrow>  ht P (afor R (j_upd, j) n m x) Q"
+  apply (hoare simp: afor_def)
+sorry
 
 lemma hl_awhile [hl_rules]: "P \<subseteq> i \<Longrightarrow> -b \<inter> i \<subseteq> Q \<Longrightarrow> ht (b \<sqinter> i) x i \<Longrightarrow> ht P (awhile i b x) Q"
   by (hoare simp: awhile_def first: hl_conseq hl: hl_while) force
